# Метод вариации произвольной постоянной для решения неоднородных линейных систем

## Метод вариации

$(1) \dot X =A(t)X+B(t)$

$\dot X=AX, \ X(t)=M(t)C$

$]X(t) = M(t)*C(t)\Rightarrow(1)$

$\dot{X}=\dot{M}(t)C(t)+M(t)\dot{C}(t)$

$\dot M(t)C(t)+M(t)\dot C(t)=AM(t)C(t)+B(t)$

$\dot{M}(t)=AM(t)$

$\cancel{AM(t)C(t)}+M(t)\dot{C}(t)=\cancel{AM(t)C(t)}+B(t)$

$M(t)\dot{C}(t)=B(t)$

$$detM=W\neq0\\\underline{\dot{C}(t)=M^{-1}(t)B(t)}\\$$

$\text{I})\dot{X}=AX+B-\text{общее решение}\\
C(t)=\int M^{-1}(t)\\
X(t)= M(t)C_0 +M(t)*\int M^{-1}(t)B(t)dt\\
\overset{o}X(t)-M(t)C_0\\
\overset{*}X(t)-\int M^{-1}(t)B(t)dt$

$$ \text{II})
\left\{\begin{aligned} 
 \dot{X}=AX+B\\
 \dot{X}_{|t=t_0}=X_0
\end{aligned} (1)\right.\\
C(t)=\int_{t0}^t M^{-1}(\tau)B(\tau)d\tau
$$

$$
X(t)=M(t)*\int_{t_0}^tM^{-1}(\tau)B(\tau)d\tau -\text{Решение задачи Коши}
$$

## Пример:

$$
\left\{\begin{aligned} 
 \dot x=x-y+1/\sqrt{\frac{1}{t}}\\
 \dot y= -2x+2y+\sqrt{\frac{1}{t}}
 \end{aligned} (2)\right.\\
A=\begin{pmatrix}
   1&-1\\
   -2&2 
\end{pmatrix}
B(t)= \begin{pmatrix}
    t^{\frac{-1}{2}}\\
    t^{\frac{-1}{2}}
\end{pmatrix}
$$

$$
det(A-\lambda I)=
\begin{vmatrix}
    1-\lambda&-1\\
    -2&2-\lambda
\end{vmatrix}=
(1-\lambda)(2-\lambda)-2=
$$

$$\Leftrightarrow \lambda^2-3\lambda=0 \Leftrightarrow\lambda(\lambda -3)=0$$

$$
\Leftrightarrow \sigma(A)=\{\lambda_1=0(k_1=1);\lambda_2=3(k_2=1)\}
$$

$$
(A-\lambda_1I)h_1=\mathbb{O} \Leftrightarrow 
\begin{pmatrix}
    1&-1\\
    -2&2
\end{pmatrix},
\sim (1\ \ -1)
$$

$$
\Rightarrow h_1{\begin{pmatrix}1\\1\end{pmatrix}}
$$

$$
(A-\lambda_2I)h_2=\mathbb{O} \Leftrightarrow 
\begin{pmatrix}
    -2&-1\\
    -2&-1
\end{pmatrix},\sim (2\ \ 1)
$$

$$
2x_1=-x_2\Leftrightarrow x_2=-2x_1,x_1=\alpha\neq 0 
$$

$$
\Rightarrow h_2{\begin{pmatrix}1\\-2\end{pmatrix}}
$$

$$
\overset{o}X(t)=C_1
\begin{pmatrix}1\\1\end{pmatrix}
+C_2*e^{3t}
\begin{pmatrix}1\\-2\end{pmatrix}
$$

$$
X_1(t)=C_1
\begin{pmatrix}1\\1\end{pmatrix}
$$

$$
X_2(t)=C_2*e^{3t}
\begin{pmatrix}1\\-2\end{pmatrix}
$$

$$
M(t)=
\begin{pmatrix}
    1&e^{3t}\\1&-2e^{3t}
\end{pmatrix};
W=-2^{3t}-e^{3t}=-3e^{3t}\neq 0
$$

$$
M^{-1}(t)=-1/3e^{-3t}
\begin{pmatrix}
    -2e^{3t}&-e^{3t}\\
    -1&1
\end{pmatrix}=
\begin{pmatrix}
    \frac{2}{3}&\frac{1}{3}\\
    \frac{1}{3}e^{-3t}&\frac{-1}{3}e^{-3t}
\end{pmatrix}
$$

$$
M^{-1}(t)B(t)=
\begin{pmatrix}
    \frac{2}{3}&\frac{1}{3}\\
    \frac{1}{3}e^{-3t}&\frac{-1}{3}e^{-3t}
\end{pmatrix}
\begin{pmatrix}t^{\frac{-1}{2}}\\t^{\frac{-1}{2}}\end{pmatrix}=
\begin{pmatrix}t^{\frac{-1}{2}}\\0\end{pmatrix}
$$

$$
\int 
\begin{pmatrix}t^{\frac{-1}{2}}\\0\end{pmatrix}dt
+C_0= 
\begin{pmatrix}2\sqrt{t}\\1\end{pmatrix}
+C_0=
$$

$$
\begin{pmatrix}2\sqrt{t}+e^{3t}\\2\sqrt{t}-2e^{3t}\end{pmatrix}+
C_1^0
\begin{pmatrix}1\\1\end{pmatrix}+C_2^0e^{3t}
\begin{pmatrix}1\\-2\end{pmatrix}
$$

$$
\begin{pmatrix}x(t)\\y(t)\end{pmatrix}=
C_1^0\begin{pmatrix}1\\1\end{pmatrix}+C_2e^{3t}
\begin{pmatrix}1\\-2\end{pmatrix}+
\begin{pmatrix}2\sqrt{t}+e^{3t}\\2\sqrt{t}-2e^{3t}\end{pmatrix}
$$
